\documentclass{article}
\begin{document}
\begin{eqnarray*}
A&=&\\
\mathrm{Repay}&=&\frac{\mathrm{foo}+\tau_{\mathrm{bar}}}{\mathrm{Loans}+ t }\\
\mathrm{bar}_2^3&=&\\
\mathrm{catching}&=&\exp\left(\left(\mathrm{Loans}+ t -\left(\mathrm{foo}+\tau_{\mathrm{bar}}\right)\right)\times b\right)\\
\mathrm{foo}&=&\mathrm{bar}\\
\mathrm{foo}_1&=&\\
\frac{ d F}{dt} &=&\mathrm{foo}\times  t \\
\frac{ d \mathrm{Loans}}{dt} &=&A+\mathrm{Repay}-\mathrm{catching}\\
\frac{ d b}{dt} &=&-\mathrm{Repay}+\mathrm{catching}\\
\end{eqnarray*}
\end{document}
